theories/rules/rules_base.v
@@ -1,14 +1,19 @@
 From machine_program_logic.program_logic Require Import weakestpre.
-From HypVeri.algebra Require Import base token reg pagetable.
+From HypVeri.algebra Require Import base reg pagetable.
 From HypVeri Require Import lifting.
 From HypVeri.lang Require Import lang_extra.
 Require Import stdpp.fin.
+
 
 Global Instance hyp_irisG `{HypervisorParameters} `{!gen_VMG Σ} :
   irisG hyp_machine Σ:=
   {
   iris_invG := gen_invG;
-  state_interp := gen_vm_interp
+  irisG_saved_prop := gen_saved_propG;
+  irisG_prop_name := gen_prop_nameG;
+  irisG_name_map := gen_name_mapG;
+  irisG_name_map_name := gen_name_map_name;
+  state_interp :=gen_vm_interp
   }.
 
 Section rules_base.
@@ -24,16 +29,35 @@ Implicit Type w: Word.
 Implicit Type q : Qp.
 
 
+(* why cannot coq figure out hyp_machine itself? *)
+Lemma just_scheduled_no_step_false{M} σ (i:nat) : @just_scheduled M σ σ i = false.
+Proof.
+  rewrite /just_scheduled /scheduled /= /scheduler.
+  apply andb_negb_l.
+Qed.
+
+Lemma just_scheduled_vms_no_step_empty{M} σ n: @just_scheduled_vms M n σ σ = [].
+Proof.
+  unfold just_scheduled_vms.
+  induction (seq 0 n);[done|].
+  rewrite filter_cons_False.
+  apply IHl.
+  rewrite just_scheduled_no_step_false //.
+Qed.
+
 Lemma not_valid_pc {a i s} :
   (to_pid_aligned a) ∉ s ->
-  {SS{{ ▷ (PC @@ i ->r a) ∗ ▷ A@i:={1}[s] }}} ExecI @ i {{{ RET FailI; PC @@ i ->r a ∗ A@i:={1}[s] }}}.
+  {SS{{ ▷ (PC @@ i ->r a) ∗ ▷ A@i:={1}[s] }}} ExecI @ i {{{ RET (false, FailI); PC @@ i ->r a ∗ A@i:={1}[s] }}}.
 Proof.
   simpl.
   iIntros (Hmm ϕ) "(>Hpc & >Ha) Hϕ".
   iApply (sswp_lift_atomic_step ExecI);[done|].
-  iIntros (σ1) "%Hsche Hσ1".
-  inversion Hsche as [ Hcur ]; clear Hsche.
-  apply fin_to_nat_inj in Hcur.
+  iIntros (n σ1) "%Hsche Hσ1".
+  rewrite /scheduled /= /scheduler /Is_true in Hsche.
+  case_match;[|done]. 
+  apply bool_decide_eq_true in Heqb.
+  apply fin_to_nat_inj in Heqb.
+  rename Heqb into Hcur.
   iModIntro.
   iDestruct "Hσ1" as "(? & ? & Hreg & ? & ? & ? & ? & Haccess & ?)".
   iDestruct (gen_reg_valid1 PC i a Hcur with "Hreg Hpc") as "%Hpc".
@@ -49,12 +73,15 @@ Proof.
     rewrite Hnacc.
     done.
   - iModIntro.
-    iIntros (m2 σ2) "%HstepP".
+    iIntros (m2 σ2) "? %HstepP".
     iModIntro.
     inversion HstepP; subst.
     + simpl.
       rewrite /gen_vm_interp.
       iFrame.
+      rewrite just_scheduled_vms_no_step_empty.
+      iSplitR;[done|].
+      rewrite andb_false_intro2;auto.
       iApply "Hϕ".
       iFrame.
     + simplify_eq.
@@ -65,6 +92,7 @@ Proof.
       inversion H.
 Qed.
 
+(* 
 Lemma eliminate_wrong_token {i j q E} :
   j ≠ i ->
   {SS{{ ▷ (<<j>>{ q })}}} ExecI @ i ; E {{{ RET ExecI ; <<j>>{ q } ∗ False }}}.
@@ -77,7 +105,6 @@ Proof.
   iExFalso.
   iPureIntro.
   done.
-Qed.
-
+Qed. *)
 
 End rules_base.
